SystemFD/Metatheory/Progress2.lean
@@ -1,0 +1,453 @@
+
+import SystemFD.Term
+import SystemFD.Ctx
+import SystemFD.Judgment
+import SystemFD.Metatheory.Classification
+import SystemFD.Metatheory.FrameWf
+import SystemFD.Reduction
+
+inductive Val : Ctx Term -> Term -> Prop where
+| app : t.neutral_form = .some (n, ts)
+      -> (Γ.is_stable_red n)
+      -> Val Γ t
+| lam :  Val Γ (`λ[a] b)
+| lamt : Val Γ (Λ[A] b)
+| refl : Val Γ (refl! _)
+| star : Val Γ ★
+| arr :  Val Γ (A -t> B)
+| arrk : Val Γ (A -k> B)
+| all : Val Γ (∀[A]B)
+| eq : Val Γ (A ~ B)
+
+theorem val_sound_var_lemma :
+  t.neutral_form = .some (n, sp) ->
+  Γ.is_stable_red n ->
+  ∀ t', ¬ (Red Γ t t')
+:= by
+intro j1 j2 t' r
+induction t generalizing n sp Γ t'
+all_goals (try simp at j1)
+case _ x =>
+  cases j1; case _ e1 e2 =>
+    subst e1; subst e2
+    cases r
+    case _ x' sp' ix tl q1 q2 q3 q4 q5 =>
+      replace q1 := Frame.is_openm_destruct q1
+      cases q1; case _ q1 =>
+        simp at *; cases q4; case _ e1 e2 =>
+          subst e1; subst e2
+          unfold Frame.is_stable_red at j2
+          simp at j2; rw [q1] at j2; simp at j2
+    case _ s x' sp' t q1 q2 =>
+      simp at *; cases q2; case _ e1 e2 =>
+        subst e1; subst e2
+        rw [<-q1] at j2; unfold Frame.is_stable_red at j2
+        simp at j2
+case _ v t1 t2 ih1 ih2 =>
+  cases v; all_goals (try simp at j1)
+  case _ =>
+    rw [Option.bind_eq_some] at j1; simp at j1
+    cases j1; case _ a j1 =>
+    cases j1; case _ b j1 =>
+    cases j1; case _ h1 h2 =>
+    cases h2; case _ h2 h3 =>
+      subst h2; cases r <;> simp at *
+      case _ x sp' ix tl q1 q2 q3 q4 q5 =>
+        replace q4 := Eq.symm q4
+        rw [Option.bind_eq_some] at q4; simp at q4
+        cases q4; case _ u q4 =>
+        cases q4; case _ v q4 =>
+        cases q4; case _ w1 w2 =>
+        cases w2; case _ w2 w3 =>
+          subst w2; rw [w1] at h1
+          injection h1 with e
+          injection e with e1 e2
+          subst e1; subst e2
+          replace q1 := Frame.is_openm_destruct q1
+          cases q1; case _ q1 =>
+            rw [q1] at j2; unfold Frame.is_stable_red at j2
+            simp at j2
+      case _ s x sp' t q1 q2 =>
+        replace q2 := Eq.symm q2
+        rw [Option.bind_eq_some] at q2; simp at q2
+        cases q2; case _ u q2 =>
+        cases q2; case _ v q2 =>
+        cases q2; case _ w1 w2 =>
+        cases w2; case _ w2 w3 =>
+          subst w2; rw [w1] at h1
+          injection h1 with e
+          injection e with e1 e2
+          subst e1; subst e2
+          rw [<-q1] at j2; unfold Frame.is_stable_red at j2
+          simp at j2
+  case _ =>
+    rw [Option.bind_eq_some] at j1; simp at j1
+    cases j1; case _ a j1 =>
+    cases j1; case _ b j1 =>
+    cases j1; case _ h1 h2 =>
+    cases h2; case _ h2 h3 =>
+      subst h2; cases r <;> simp at *
+      case _ x sp' ix tl q1 q2 q3 q4 q5 =>
+        replace q4 := Eq.symm q4
+        rw [Option.bind_eq_some] at q4; simp at q4
+        cases q4; case _ u q4 =>
+        cases q4; case _ v q4 =>
+        cases q4; case _ w1 w2 =>
+        cases w2; case _ w2 w3 =>
+          subst w2; rw [w1] at h1
+          injection h1 with e
+          injection e with e1 e2
+          subst e1; subst e2
+          replace q1 := Frame.is_openm_destruct q1
+          cases q1; case _ q1 =>
+            rw [q1] at j2; unfold Frame.is_stable_red at j2
+            simp at j2
+      case _ s x sp' t q1 q2 =>
+        replace q2 := Eq.symm q2
+        rw [Option.bind_eq_some] at q2; simp at q2
+        cases q2; case _ u q2 =>
+        cases q2; case _ v q2 =>
+        cases q2; case _ w1 w2 =>
+        cases w2; case _ w2 w3 =>
+          subst w2; rw [w1] at h1
+          injection h1 with e
+          injection e with e1 e2
+          subst e1; subst e2
+          rw [<-q1] at j2; unfold Frame.is_stable_red at j2
+          simp at j2
+      case _ tl r e => apply ih1 h1 j2 tl r
+  case _ =>
+    rw [Option.bind_eq_some] at j1; simp at j1
+    cases j1; case _ a j1 =>
+    cases j1; case _ b j1 =>
+    cases j1; case _ h1 h2 =>
+    cases h2; case _ h2 h3 =>
+      subst h2; cases r <;> simp at *
+      case _ x sp' ix tl q1 q2 q3 q4 q5 =>
+        replace q4 := Eq.symm q4
+        rw [Option.bind_eq_some] at q4; simp at q4
+        cases q4; case _ u q4 =>
+        cases q4; case _ v q4 =>
+        cases q4; case _ w1 w2 =>
+        cases w2; case _ w2 w3 =>
+          subst w2; rw [w1] at h1
+          injection h1 with e
+          injection e with e1 e2
+          subst e1; subst e2
+          replace q1 := Frame.is_openm_destruct q1
+          cases q1; case _ q1 =>
+            rw [q1] at j2; unfold Frame.is_stable_red at j2
+            simp at j2
+      case _ s x sp' t q1 q2 =>
+        replace q2 := Eq.symm q2
+        rw [Option.bind_eq_some] at q2; simp at q2
+        cases q2; case _ u q2 =>
+        cases q2; case _ v q2 =>
+        cases q2; case _ w1 w2 =>
+        cases w2; case _ w2 w3 =>
+          subst w2; rw [w1] at h1
+          injection h1 with e
+          injection e with e1 e2
+          subst e1; subst e2
+          rw [<-q1] at j2; unfold Frame.is_stable_red at j2
+          simp at j2
+      case _ tl r e => apply ih1 h1 j2 tl r
+
+theorem val_sound : Val Γ t -> ∀ t', ¬ (Red Γ t t') := by
+intro j; induction j
+case _ Γ t n sp j2 j3 =>
+  intro t' r
+  apply val_sound_var_lemma j2 j3 t' r
+all_goals (
+  case _ =>
+    intro t' r
+    cases r <;> simp at *
+)
+
+@[simp]
+abbrev TypesAreValuesLemmaType : (v : JudgmentVariant) -> (Γ : Ctx Term) -> (JudgmentArgs v) -> Prop
+| .prf => λ Γ => λ(t , K) => Γ ⊢ K : .kind -> Val Γ t
+| .wf  => λ _ => λ () => true
+
+theorem types_are_values_lemma :
+  Judgment v Γ ix ->
+  TypesAreValuesLemmaType v Γ ix
+:= by
+intro j; induction j <;> simp at *
+all_goals (intro h1)
+case _ j _ _ _ _ =>
+  have lem := uniqueness_of_types j h1
+  injection lem
+case _ => cases h1
+case _ Γ x T j1 j2 _ =>
+  generalize fdef : Γ d@ x = f at *
+  have lem := frame_wf_by_index x j1
+  rw [fdef] at lem
+  cases lem
+  all_goals (
+    unfold Frame.get_type at j2
+    simp at j2
+  )
+  case type j3 =>
+    subst j2
+    have lem := uniqueness_of_types h1 j3
+    injection lem
+  case openm j3 =>
+    subst j2
+    have lem := uniqueness_of_types h1 j3
+    injection lem
+  case term j3 _ =>
+    subst j2
+    have lem := uniqueness_of_types h1 j3
+    injection lem
+  all_goals (
+    case _ =>
+      subst j2; apply @Val.app Γ #x x []
+      simp; simp; rw [fdef]; unfold Frame.is_stable_red
+      simp
+  )
+case _ => cases h1
+case _ => apply Val.all
+case _ => apply Val.arr
+case _ Γ f A B a j1 j2 ih1 ih2 =>
+  have lem := classification_lemma j1 <;> simp at lem
+  cases lem
+  case _ lem =>
+    replace ih1 := ih1 lem
+    cases ih1
+    case app x sp q1 q2 =>
+      apply @Val.app Γ (f `@k a) x (sp ++ [(.kind, a)])
+      simp; rw [Option.bind_eq_some]; simp; apply q2
+      apply q1
+    all_goals (cases j1)
+  case _ lem =>
+    cases lem; case _ K lem =>
+      cases lem.2; cases lem.1
+case _ => apply Val.eq
+case _ j _ _ _ _ _ _ _ =>
+  have lem := uniqueness_of_types j h1
+  injection lem
+case _ j _ _ _ _ _ =>
+  have lem := uniqueness_of_types j h1
+  injection lem
+case _ => apply Val.lam
+case _ Γ f A B a B' j1 j2 j3 ih1 ih2 =>
+  have lem := classification_lemma j1
+  cases lem <;> simp at *
+  case _ lem =>
+    cases lem <;> simp at *
+    case _ lem => cases lem
+    case _ lem =>
+      cases lem; case _ K lem =>
+      cases lem.2; case _ j4 j5 =>
+        replace j5 := beta_empty a j5; simp at j5
+        rw [j3] at h1
+        have lem := uniqueness_of_types h1 j5
+        injection lem
+case _ => apply Val.lamt
+case _ Γ f A B a B' j1 j2 j3 ih1 ih2 =>
+  have lem := classification_lemma j1
+  cases lem <;> simp at *
+  case _ lem =>
+    cases lem <;> simp at *
+    case _ lem => cases lem
+    case _ lem =>
+      cases lem; case _ K lem =>
+      cases lem.2; case _ j4 j5 =>
+        replace j5 := beta_kind j5 j2; simp at j5
+        rw [j3] at h1
+        have lem := uniqueness_of_types h1 j5
+        injection lem
+case _ j _ _ =>
+  have lem := classification_lemma j <;> simp at lem
+  cases lem
+  case _ lem => cases lem
+  case _ lem =>
+    cases lem; case _ K lem =>
+    cases lem.2; case _ q _ j2 =>
+      have lem2 := uniqueness_of_types h1 j2
+      subst lem2; cases q
+case _ => apply Val.refl
+all_goals (case _ => cases h1)
+
+theorem types_are_values :
+  Γ ⊢ t : K ->
+  Γ ⊢ K : .kind ->
+  Val Γ t
+:= by
+intro j1 j2
+apply types_are_values_lemma j1 j2
+
+@[simp]
+abbrev ProgressLemmaType : (v : JudgmentVariant) -> (Γ : Ctx Term) -> (JudgmentArgs v) -> Prop
+| .prf => λ Γ => λ(t , _) => Val Γ t ∨ ∃ t', Red Γ t t'
+| .wf  => λ _ => λ () => true
+
+theorem progress_lemma :
+  (∀ x, ¬ Γ.is_type x) ->
+  Judgment v Γ ix ->
+  ProgressLemmaType v Γ ix
+:= by
+intro h1 j
+induction j <;> try simp at *
+case _ =>
+  apply Or.inr; apply Exists.intro _
+  apply Red.letbeta
+case _ => apply Or.inl; apply Val.star
+case _ Γ x T j1 j2 _ =>
+  generalize fdef : Γ d@ x = f at *
+  cases f
+  case term A t =>
+    apply Or.inr; apply Exists.intro _
+    apply @Red.letterm A #x x [] Γ t
+    simp; rw [fdef]
+  case openm A =>
+    let indices := instance_indices Γ 0 x []
+    let insts := get_instances Γ indices
+    apply Or.inr; apply Exists.intro insts
+    apply @Red.inst #x x [] indices Γ insts
+    simp; simp; rw [fdef]; unfold Frame.is_openm; simp
+    simp; simp; simp
+  case type =>
+    replace h1 := h1 x
+    rw [fdef] at h1; unfold Frame.is_type at h1
+    simp at h1
+  case empty =>
+    unfold Frame.get_type at j2; simp at j2
+  all_goals (
+    apply Or.inl; apply @Val.app Γ #x x []
+    simp; simp; unfold Frame.is_stable_red
+    rw [fdef]
+  )
+case _ => apply Or.inl; apply Val.arrk
+case _ => apply Or.inl; apply Val.all
+case _ => apply Or.inl; apply Val.arr
+case _ Γ f A B a j1 j2 ih1 ih2 =>
+  have lem := classification_lemma j1; simp at lem
+  cases lem
+  case _ lem =>
+    have lem2 := types_are_values j1 lem
+    cases lem2
+    case app x sp q1 q2 =>
+      apply Or.inl; apply @Val.app Γ (f `@k a) x (sp ++ [(.kind, a)])
+      simp; rw [Option.bind_eq_some]; simp; apply q2
+      apply q1
+    all_goals (cases j1)
+  case _ lem =>
+    cases lem; case _ K lem =>
+    cases lem.2; cases lem.1
+case _ => apply Or.inl; apply Val.eq
+case _ Γ p A s R i B T e j1 j2 j3 j4 j5 j6 j7 j8 j9 j10 ih1 ih2 ih3 ih4 ih5 ih6 =>
+  replace ih2 := ih2 h1
+  cases ih2
+  case _ h2 =>
+    apply Or.inr
+    unfold ValidHeadVariable at j5
+    unfold ValidHeadVariable at j6
+    cases j5; case _ w1 j5 =>
+    cases w1; case _ w1 sp1 =>
+    cases j6; case _ w2 j6 =>
+    cases w2; case _ w2 sp2 =>
+      simp at j5; simp at j6
+      cases h2
+      case _ x sp3 q2 q3 =>
+        generalize tstdef : prefix_equal sp1 sp3 = tst
+        cases tst
+        case _ =>
+          apply Exists.intro _
+          apply Red.ite_missed j5.1 (Eq.symm q3) q2 (Or.inr tstdef)
+        case _ ξ =>
+          cases (Nat.decEq w1 x)
+          case _ h =>
+            apply Exists.intro _
+            apply Red.ite_missed j5.1 (Eq.symm q3) q2 (Or.inl h)
+          case _ h =>
+            subst h; apply Exists.intro _
+            apply Red.ite_matched j5.1 (Eq.symm q3) (Eq.symm tstdef) j5.2
+      all_goals (cases j2; simp at j6)
+  case _ h2 =>
+    cases h2; case _ s' h2 =>
+      apply Or.inr
+      apply Exists.intro (List.map (fun x => p.ite x i e) s')
+      apply Red.ite_congr h2; rfl
+case _ Γ p A s R t B T j1 j2 j3 j4 j5 j6 j7 j8 j9 ih1 ih2 ih3 ih4 ih5 =>
+  replace ih2 := ih2 h1
+  cases ih2
+  case _ h2 =>
+    apply Or.inr
+    unfold ValidHeadVariable at j5
+    unfold ValidHeadVariable at j6
+    cases j5; case _ w1 j5 =>
+    cases w1; case _ w1 sp1 =>
+    cases j6; case _ w2 j6 =>
+    cases w2; case _ w2 sp2 =>
+      simp at j5; simp at j6
+      cases h2
+      case _ x sp3 q2 q3 =>
+        generalize tstdef : prefix_equal sp1 sp3 = tst
+        cases tst
+        case _ =>
+          apply Exists.intro _
+          apply Red.guard_missed j5.1 (Eq.symm q3) q2 (Or.inr tstdef)
+        case _ ξ =>
+          cases (Nat.decEq w1 x)
+          case _ h =>
+            apply Exists.intro _
+            apply Red.guard_missed j5.1 (Eq.symm q3) q2 (Or.inl h)
+          case _ h =>
+            subst h; apply Exists.intro [t.apply_spine ξ]
+            apply @Red.guard_matched p w1 sp1 s sp3 ξ Γ t
+            apply j5.1; apply Eq.symm q3
+            apply Eq.symm tstdef
+      all_goals (cases j2; simp at j6)
+  case _ h2 =>
+    cases h2; case _ s' h2 =>
+      apply Or.inr
+      apply Exists.intro (List.map (fun x => p.guard x t) s')
+      apply Red.guard_congr h2; rfl
+case _ => apply Or.inl; apply Val.lam
+case _ Γ f A B a B' j1 j2 j3 ih1 ih2 =>
+  replace ih1 := ih1 h1
+  cases ih1
+  case _ h2 =>
+    cases h2
+    case app x sp q1 q2 =>
+      apply Or.inl; apply @Val.app Γ (f `@ a) x (sp ++ [(.term, a)])
+      simp; rw [Option.bind_eq_some]; simp; apply q2
+      apply q1
+    case lam =>
+      apply Or.inr; apply Exists.intro _
+      apply Red.beta
+    all_goals (cases j1)
+  case _ h2 =>
+    cases h2; case _ f' h2 =>
+      apply Or.inr; apply Exists.intro (List.map (· `@ a) f')
+      apply Red.app_congr h2 rfl
+case _ => apply Or.inl; apply Val.lamt
+case _ Γ f A B a B' j1 j2 j3 ih1 ih2 =>
+  replace ih1 := ih1 h1
+  cases ih1
+  case _ h2 =>
+    cases h2
+    case app x sp q1 q2 =>
+      apply Or.inl; apply @Val.app Γ (f `@t a) x (sp ++ [(.type, a)])
+      simp; rw [Option.bind_eq_some]; simp; apply q2
+      apply q1
+    case lamt =>
+      apply Or.inr; apply Exists.intro _
+      apply Red.betat
+    all_goals (cases j1)
+  case _ h2 =>
+    cases h2; case _ f' h2 =>
+      apply Or.inr; apply Exists.intro (List.map (· `@t a) f')
+      apply Red.appt_congr h2 rfl
+case _ => sorry
+case _ => apply Or.inl; apply Val.refl
+case _ => sorry
+case _ => sorry
+case _ => sorry
+case _ => sorry
+case _ => sorry
+case _ => sorry
+case _ => sorry
+case _ => sorry
